WIP proof forward_nl missing

verif_tweetnacl.v
@@ -1,4 +1,5 @@
 Require Import floyd.proofauto. (* Import the Verifiable C system *)
+
 Require Import tweetnacl. (* Import the AST of this C program *)
 (* The next line is "boilerplate", always required after importing an AST. *)
 Instance CompSpecs : compspecs. make_compspecs prog. Defined.
@@ -9,22 +10,23 @@ Require Import arith.
 
 
 (* Beginning of the API spec for the sumarray.c program *)
-Definition A_spec n :=
+Definition A_spec :=
  DECLARE _A
   WITH i: val, o: val, a: val, b: val, sh : share, contents_o : list Z, contents_a : list Z, contents_b : list Z
   PRE [ _o OF (tptr tlong), _a OF (tptr tlong), _b OF (tptr tlong) ]
         PROP  (readable_share sh;
-                Forall (fun x => 0 <= x <= Z.pow 2 n) contents_a;
-                Forall (fun x => 0 <= x <= Z.pow 2 n) contents_b;
-                length contents_a = 16;
-                length contents_b = 16)
+                Forall (fun x => 0 <= x < Z.pow 2 63) contents_a;
+                Forall (fun x => 0 <= x < Z.pow 2 63) contents_b;
+                length contents_a = 16%nat;
+                length contents_b = 16%nat;
+                length contents_o = 16%nat)
         LOCAL (temp _i i)
         SEP   (data_at sh (tarray tlong 16) (map Vlong (map Int64.repr contents_a)) a;
               data_at sh (tarray tlong 16) (map Vlong (map Int64.repr contents_b)) b;
               data_at sh (tarray tlong 16) (map Vlong (map Int64.repr contents_o)) o)
   POST [ tvoid ]
         PROP (readable_share sh;
-                Forall (fun x => 0 <= x <= Z.pow 2 (Z.succ n)) contents_o)
+                Forall (fun x => 0 <= x < Z.pow 2 (Z.succ 63)) contents_o)
         LOCAL()
         SEP (data_at sh (tarray tlong 16) (map Vlong (map Int64.repr contents_a)) a;
               data_at sh (tarray tlong 16) (map Vlong (map Int64.repr contents_b)) b;
@@ -34,21 +36,75 @@ Definition A_spec n :=
   Then the [Forall] would not be needed in the PROP part of PRE.
 *)
 
-Definition A_Inv sh a b contents_a contents_b := 
-   PROP  ()
+Definition A_Inv sh o a b contents_o contents_a contents_b := 
+  EX i : Z,
+   PROP  (i >= 0; sum_list_Z_n (nat_of_Z i) contents_a contents_b = slice (nat_of_Z i) contents_o)
    LOCAL ()
-   SEP   (data_at sh (tarray tlong 16) (map Vlong (map Int64.repr contents_a)) a;
+   SEP   (data_at sh (tarray tlong 16) (map Vlong (map Int64.repr contents_o)) o;
+          data_at sh (tarray tlong 16) (map Vlong (map Int64.repr contents_a)) a;
           data_at sh (tarray tlong 16) (map Vlong (map Int64.repr contents_b)) b).
+
+Lemma SumListForall : forall n a b c,
+  n > 0 ->
+  Forall (fun x : Z => 0 <= x < 2 ^ n) a ->
+  Forall (fun x : Z => 0 <= x < 2 ^ n) b ->
+  sum_list_Z a b = c ->
+  Forall (fun x : Z => 0 <= x < 2 ^ (Z.succ n)) c.
+Proof.
+induction n ; [intros | | intros; assert(Hp:=Zlt_neg_0)] ; go.
+assert(Hp: exists n, n = Z.pos p) by (exists (Z.pos p); reflexivity); destruct Hp as [n Hp].
+rewrite <- Hp in *.
+assert(Hfa: forall a, 0 <= a < 2^n -> 0 <= a < 2^Z.succ n).
+intros x Hx ; split ; destruct Hx ; auto ; rewrite Z.pow_succ_r ; assert(Hpp:= Zgt_pos_0 p) ; rewrite <- Hp in Hpp ; omega.
+induction a,b ; intros c Hn Ha Hb Hsum ; simpl in Hsum ; subst c ; auto.
+- eapply (Forall_impl (fun x : Z => 0 <= x < 2 ^ Z.succ n) Hfa) ; auto.
+- eapply (Forall_impl (fun x : Z => 0 <= x < 2 ^ Z.succ n) Hfa) ; auto.
+  apply Forall_cons.
+  {
+  inv Ha.
+  inv Hb.
+  destruct H1.
+  destruct H3.
+  split ; try omega.
+  apply addition ; try omega.
+  }
+  {
+  apply (IHa b); auto.
+  inv Ha ; auto.
+  inv Hb ; auto.
+  }
+Qed.
 
 
 (* Packaging the API spec all together. *)
-Definition Gprog n  : funspecs := 
-      augment_funspecs prog [A_spec n].
+Definition Gprog : funspecs := 
+      augment_funspecs prog [A_spec].
+
 
 (** Proof that f_sumarray, the body of the sumarray() function,
  ** satisfies sumarray_spec, in the global context (Vprog,Gprog).
  **)
-Lemma body_sumarray n: semax_body Vprog (Gprog n) f_A (A_spec n).
+Lemma body_sumarray: semax_body Vprog Gprog f_A A_spec.
 Proof.
 start_function.
-forward.
+forward_for_simple_bound 16 (A_Inv sh o a b contents_o contents_a contents_b).
+
+- go_lowerx.
+  entailer!.
+  flatten.
+- admit. (* apply semax_loadstore_array. forward.*)
+
+- normalize.
+  change (nat_of_Z 16) with (16%nat) in H5.
+  rewrite <- sum_list_eq in H5 ; go.
+  rewrite slice_length_eq in H5 ; go.
+  rewrite <- H5.
+  forward.
+  assert(HSum:= SumListForall 63 contents_a contents_b (sum_list_Z contents_a contents_b)).
+  assert(HSum': 63 > 0) by omega.
+  apply HSum in HSum'.
+  entailer!.
+  apply H.
+  apply H0.
+  auto.
+Qed.
